$$
\begin{align}
&1+r+r^{2}+\cdots+r^{n}=\frac{1-r^{n+1}}{1-r}\quad (r\neq 1) \\
&1+(-x^{2})+(-x^{2})^{2}+\cdots+(-x^{2})^{n}=\frac{1+x^{2n+2}}{1+x^{2}}\quad \\
&\frac{1}{1+x^{2}}+\frac{x^{2n+2}}{1+x^{2}}=1-x^{2}+x^{4}+\cdots x^{2n} \\
&\frac{1}{1+x^{2}}=1-x^{2}+x^{4}+\cdots x^{2n}-\frac{x^{2n+2}}{1+x^{2}} 
\end{align}

$$
이를 $[0, x]$에 대해 적분하면 (단, $0\leq x\leq 1$)
$$
\int_{0}^{x} \frac{1}{1+t^{2}}  \, dt =x-\frac{1}{3}x^{3}+\frac{1}{5}x^{5}\cdots+\frac{1}{2n+1}x^{2n+1}-\int_{0}^{x} \frac{t^{2n+2}}{1+t^{2}} \, dt
$$
이때 
$$
0\leq \int_{0}^{a} \frac{t^{2n+2}}{1+t^{2}} \, dx\leq \int_{0}^{a} t^{2n+2} \, dx \leq \frac{1}{2n+3}
$$
이므로
$$
\begin{align}
\int_{0}^{x} \frac{1}{1+t^{2}}  \, dt &=\lim_{ n \to \infty } (x-\frac{1}{3}x^{3}+\frac{1}{5}x^{5}\cdots+\frac{1}{2n+1}x^{2n+1}) \\
\tan^{-1}x &=\lim_{ n \to \infty } (x-\frac{1}{3}x^{3}+\frac{1}{5}x^{5}\cdots+\frac{1}{2n+1}x^{2n+1}) \\
\therefore \frac{\pi}{4}&=1-\frac{1}{3}^{3}+\frac{1}{5}^{5}\cdots+\frac{1}{2n+1}\quad(x=1)
\end{align}
$$
$$
L:= \sum_{k=1}^{\infty} \frac{(-1)^{k+1}}{2k-1}=\frac{\pi}{4}
$$
