## 1 곱미분
$$
\begin{align}
F(x)&=f(x)g(x) \\
F'(x)&=\lim_{ h \to 0 } \frac{{F(x+h)-F(x)}}{h} \\
&=\lim_{ h \to 0 } \frac{{f(x+h)g(x+h)-f(x)g(x)}}{h} \\
&=\lim_{ h \to 0 } \frac{{f(x+h)g(x+h)-f(x+h)g(x)+f(x+h)g(x)-f(x)g(x)}}{h} \\
&=\lim_{ h \to 0 }f(x+h)\lim_{ h \to 0 }\frac{{g(x+h)-g(x)}}{h}+g(x)\lim_{ h \to 0 }\frac{{{f(x+h)-f(x)}}}{h} \\
&=f'(x)g(x)+f(x)g'(x)
\end{align}
$$
## 2 몫미분
$$
\begin{align}
F(x)=\frac{f(x)}{g(x)}\quad (g(x)\neq 0)
\end{align}
$$
$$
\begin{align}
f(x)&=F(x)g(x) \\
&=F(x)g'(x)+F'(x)g(x)
\end{align}
$$
$$
\begin{align}
F'(x)&=\frac{{f'(x)-F(x)g'(x)}}{g(x)} \\
&=\frac{{f'(x)-\frac{f(x)}{g(x)}g'(x)}}{g(x)} \\
&=\frac{{f'(x)g(x)-f(x)g'(x)}}{[g(x)]^{2}}
\end{align}
$$
$$
\therefore F'(x)=\frac{{f'(x)g(x)-f(x)g'(x)}}{[g(x)]^{2}}
$$
## 3 역함수 미분
$$
\begin{align}
f^{-1}(x)=g(x) \\
f(g(x))=x \\
f'(g(x))\cdot g'(x)=1 \\
g'(x)=\frac{1}{f'(g(x))}\tag{1} \\
\end{align}
$$
$$
\begin{align}
f(y)=x \\
f'(y) \frac{dy}{dx}=1 \\
\frac{dx}{dy}=\frac{1}{f'(y)}\tag{2} \\
\end{align}
$$
$\frac{dx}{dy}=g'(x), y=g(x)$이므로
$$
\begin{align}
g'(x)=\frac{1}{f'(g(x))}
\end{align}
$$

